major filename refactoring

src/basic/Events.v
@@ -1,62 +1,273 @@
-(******************************************************************************)
-(** * Definition of execution graph events *)
-(******************************************************************************)
+Require Import Labels.
+From hahn Require Import Hahn. 
 Require Import Lia.
-Require Import FinFun.
-Require Import List.
-From hahn Require Import Hahn.
-Require Import AuxRel.
-Require Import basic.Labels.
-
-Set Implicit Arguments.
-
-Definition Tid := nat.
-
 Section Events.
 
-(******************************************************************************)
-(** ** Execution graph events  *)
-(******************************************************************************)
+(* req + resp объединить *)
 
-Inductive Event := 
-  | InitEvent (x : Labels.Loc)
-  | ThreadEvent (thread : Tid) (index : nat) (l : Lab).
+Inductive FPGAEvent :=
+  | Fpga_write_req (c:Chan) (x:Loc) (v:Val)
+  | Fpga_read_req (c:Chan) (x:Loc)
+  | Fpga_fence_req_one (c: Chan)
+  | Fpga_fence_req_all
+  | Fpga_write_resp (c:Chan) (x:Loc) (v:Val)
+  | Fpga_read_resp (c:Chan) (x:Loc) (v:Val)
+  | Fpga_fence_resp_one (c: Chan)
+  | Fpga_fence_resp_all.
 
-Definition is_init a := 
-  match a with
+Inductive CPUEvent := 
+(*   | Askip  *)
+  | Cpu_load  (x:Loc) (v:Val)
+  | Cpu_store (x:Loc) (v:Val)
+  | Cpu_fence.
+
+Inductive Event :=
+  | ThreadEvent (thread: nat) (index: nat) (e: CPUEvent)
+  | FpgaEvent (e: FPGAEvent) (index: nat) (m: Mdata)
+  | InitEvent (x : Labels.Loc).
+
+Definition fpga_chan_opt (e: FPGAEvent) :=
+  match e with
+  | Fpga_write_req c _ _ => Some c
+  | Fpga_read_req c _ => Some c
+  | Fpga_fence_req_one c => Some c
+  | Fpga_write_resp c _ _ => Some c
+  | Fpga_read_resp c _ _ => Some c
+  | Fpga_fence_resp_one c => Some c
+  | Fpga_fence_req_all => None
+  | Fpga_fence_resp_all => None
+  end.
+
+Definition chan_opt (e: Event) :=
+  match e with
+  | ThreadEvent _ _ _ => None
+  | FpgaEvent e _ _ => fpga_chan_opt e
+  | InitEvent _ => None
+end.
+
+Definition tid (e: Event) : Tid :=
+  match e with
+  | ThreadEvent t _ _ => CpuTid t
+  | FpgaEvent _ _ _ => FpgaTid
+  | InitEvent _ => InitTid
+  end. 
+
+Definition loc (e: Event) := match e with
+  | ThreadEvent _ _ (Cpu_load x _) => x
+  | ThreadEvent _ _ (Cpu_store x _) => x
+  | ThreadEvent _ _ Cpu_fence => 0
+  | FpgaEvent (Fpga_write_req _ x _) _ _ => x
+  | FpgaEvent (Fpga_read_req _ x) _ _ => x
+  | FpgaEvent (Fpga_write_resp _ x _) _ _ => x
+  | FpgaEvent (Fpga_read_resp _ x _) _ _ => x
+  | FpgaEvent (Fpga_fence_req_one _) _ _ => 0
+  | FpgaEvent (Fpga_fence_req_all) _ _ => 0
+  | FpgaEvent (Fpga_fence_resp_one _) _ _ => 0
+  | FpgaEvent (Fpga_fence_resp_all) _ _ => 0
+  | InitEvent l => l
+  end.
+
+Definition valr (e: Event) := match e with
+  | ThreadEvent _ _ (Cpu_load _ v) => v
+  | ThreadEvent _ _ (Cpu_store _ _) => 0
+  | ThreadEvent _ _ Cpu_fence => 0
+  | FpgaEvent (Fpga_write_req _ _ v) _ _ => 0
+  | FpgaEvent (Fpga_read_req _ _) _ _ => 0
+  | FpgaEvent (Fpga_write_resp _ _ _) _ _ => 0
+  | FpgaEvent (Fpga_read_resp _ _ v) _ _ => v
+  | FpgaEvent (Fpga_fence_req_one _) _ _ => 0
+  | FpgaEvent (Fpga_fence_req_all) _ _ => 0
+  | FpgaEvent (Fpga_fence_resp_one _) _ _ => 0
+  | FpgaEvent (Fpga_fence_resp_all) _ _ => 0
+  | InitEvent _ => 0
+  end.
+
+Definition valw (e: Event) := match e with
+  | ThreadEvent _ _ (Cpu_load _ _) => 0
+  | ThreadEvent _ _ (Cpu_store _ v) => v
+  | ThreadEvent _ _ Cpu_fence => 0
+  | FpgaEvent (Fpga_write_req _ _ v) _ _ => v
+  | FpgaEvent (Fpga_read_req _ _) _ _ => 0
+  | FpgaEvent (Fpga_write_resp _ _ v) _ _ => v
+  | FpgaEvent (Fpga_read_resp _ _ _) _ _ => 0
+  | FpgaEvent (Fpga_fence_req_one _) _ _ => 0
+  | FpgaEvent (Fpga_fence_req_all) _ _ => 0
+  | FpgaEvent (Fpga_fence_resp_one _) _ _ => 0
+  | FpgaEvent (Fpga_fence_resp_all) _ _ => 0
+  | InitEvent _ => 0
+  end.
+
+Definition index(e: Event) := match e with
+  | ThreadEvent _ i _ => i
+  | FpgaEvent _ i _ => i
+  | InitEvent _ => 0
+end.
+
+Definition meta (e: Event) := match e with
+  | ThreadEvent _ _ _ => 0
+  | FpgaEvent _ _ m => m
+  | InitEvent _ => 0
+  end.
+
+
+Definition is_wr_req (e: Event) :=
+  match e with
+  | FpgaEvent (Fpga_write_req _ _ _) _ _ => True
+  | _ => False
+end.
+
+Definition is_wr_resp (e: Event) :=
+  match e with
+  | FpgaEvent (Fpga_write_resp _ _ _) _ _ => True
+  | _ => False
+end.
+
+Definition is_rd_req (e: Event) :=
+  match e with
+  | FpgaEvent (Fpga_read_req _ _) _ _ => True
+  | _ => False
+end.
+
+Definition is_rd_resp (e: Event) := 
+  match e with
+  | FpgaEvent (Fpga_read_resp _ _ _) _ _ => True
+  | _ => False
+end.
+
+Definition is_fence_req_one (e: Event) :=
+  match e with
+  | FpgaEvent (Fpga_fence_req_one _) _ _ => True
+  | _ => False
+end.
+
+Definition is_fence_resp_one (e: Event) :=
+  match e with
+  | FpgaEvent (Fpga_fence_resp_one _) _ _ => True
+  | _ => False
+end.
+
+Definition is_fence_req_all (e: Event) := 
+  match e with
+  | FpgaEvent (Fpga_fence_req_all) _ _ => True
+  | _ => False
+end.
+
+Definition is_fence_resp_all (e: Event) :=
+  match e with
+  | FpgaEvent (Fpga_fence_resp_all) _ _ => True
+  | _ => False
+end.
+
+Definition is_cpu_wr (e: Event) :=
+  match e with
+  | ThreadEvent _ _ (Cpu_store _ _) => True
+  | _ => False
+end.
+
+Definition is_cpu_rd (e: Event) :=
+  match e with
+  | ThreadEvent _ _ (Cpu_load _ _) => True
+  | _ => False
+end.
+
+Definition is_cpu_fence (e: Event) :=
+  match e with
+  | ThreadEvent _ _ (Cpu_fence) => True
+  | _ => False
+end.
+
+Definition is_init e := 
+  match e with
     | InitEvent _ => True
     | _ => False
   end.
 
-Definition tid a := 
-  match a with
-    | InitEvent _ => 0
-    | ThreadEvent i _ _ => i
+Definition is_cpu e := 
+  match e with
+    | ThreadEvent _ _ _ => True
+    | _ => False
   end.
 
-Definition index a := 
-  match a with
-    | InitEvent _ => 0
-    | ThreadEvent _ n _ => n
+Definition is_fpga e : Prop := 
+  match e with
+    | FpgaEvent _ _ _ => True
+    | _ => False
+end.
+
+Definition is_w e : Prop :=
+  match e with
+  | ThreadEvent _ _ (Cpu_store _ _) => True
+  | FpgaEvent (Fpga_write_resp _ _ _) _ _ => True
+  | InitEvent _ => True
+  | _ => False
+end.
+
+Definition is_r e : Prop :=
+  match e with
+  | ThreadEvent _ _ (Cpu_load _ _) => True
+  | FpgaEvent (Fpga_read_resp _ _ _) _ _ => True
+  | _ => False
+end.
+
+Definition is_req (e1 : Event) :=
+  match e1 with
+  | FpgaEvent (Fpga_write_req _ _ _) _ _ => True
+  | FpgaEvent (Fpga_read_req _ _) _ _ => True
+  | FpgaEvent (Fpga_fence_req_one _) _ _ => True
+  | FpgaEvent (Fpga_fence_req_all) _ _ => True
+  | _ => False
+end.
+
+Definition is_resp (e1 : Event) :=
+  match e1 with
+  | FpgaEvent (Fpga_write_resp _ _ _) _ _ => True
+  | FpgaEvent (Fpga_read_resp _ _ _) _ _ => True
+  | FpgaEvent (Fpga_fence_resp_one _) _ _ => True
+  | FpgaEvent (Fpga_fence_resp_all) _ _ => True
+  | _ => False
+end.
+
+
+
+Definition req_resp_pair (e1 e2: Event) :=
+  match e1, e2 with
+  | FpgaEvent (Fpga_write_req chan1 l1 v1) _ meta1, FpgaEvent (Fpga_write_resp chan2 l2 v2) _ meta2 => chan1 = chan2 /\ meta1 = meta2 /\ l1 = l2 /\ v1 = v2
+  | FpgaEvent (Fpga_read_req chan1 _) _ meta1, FpgaEvent (Fpga_read_resp chan2 _ _) _ meta2 => chan1 = chan2 /\ meta1 = meta2
+  | FpgaEvent (Fpga_fence_req_one chan1) _ meta1, FpgaEvent (Fpga_fence_resp_one chan2) _ meta2 => chan1 = chan2 /\ meta1 = meta2
+  | FpgaEvent (Fpga_fence_req_all) _ meta1, FpgaEvent (Fpga_fence_resp_all) _ meta2 => meta1 = meta2
+  | _, _ => False
   end.
 
-Definition lab a := 
-  match a with
-    | InitEvent x => (Astore x 0)
-    | ThreadEvent _ _ l => l
+(* Definition req_resp_pair (e1 e2 : Event) :=
+  match e1, e2 with
+  | EventLab (FpgaEvent (Fpga_read_req _ _) _ _), EventLab (FpgaEvent (Fpga_read_resp _ _ _) _ _) => True
+  | EventLab (FpgaEvent (Fpga_write_req _ _ _) _ _), EventLab (FpgaEvent (Fpga_write_resp _) _ _) => True
+  | EventLab (FpgaEvent (Fpga_fence_req_one _) _ _), EventLab (FpgaEvent (Fpga_fence_resp_one _) _ _) => True
+  | EventLab (FpgaEvent (Fpga_fence_req_all) _ _), EventLab (FpgaEvent (Fpga_fence_resp_all) _ _) => True
+  | _, _ => False
   end.
 
-Definition loc a := loc_l (lab a).
-Definition valr a := valr_l (lab a).
-Definition valw a := valw_l (lab a).
-Definition is_r a := is_r_l (lab a).
-Definition is_w a := is_w_l (lab a).
-Definition is_rmw a := is_rmw_l (lab a).
+Definition is_req e := match e with
+  | EventLab (FpgaEvent (Fpga_read_req _ _) _ _) => True
+  | EventLab (FpgaEvent (Fpga_write_req _ _ _) _ _) => True
+  | EventLab (FpgaEvent (Fpga_fence_req_one _) _ _) => True
+  | EventLab (FpgaEvent (Fpga_fence_req_all) _ _) => True
+  | _ => False
+  end.
 
-Lemma r_or_w a : is_r a \/ is_w a.
+Definition meta_pair_unique :=
+  same_meta_l ⊆ (is_pair)^?.
+
+
+(* Для каждого запроса существует пара *)
+Definition req_exists_resp :=
+  forall e1, is_req e1 -> exists e2, is_pair e1 e2. *)
+
+
+(* Lemma r_or_w a : is_r a \/ is_w a.
 Proof using.
   unfold is_r, is_w. destruct (lab a); ins; auto.
-Qed.
+Qed. *)
 
 (******************************************************************************)
 (** ** is_init properties *)
@@ -64,19 +275,29 @@ Qed.
 Lemma is_init_InitEvent x :
   is_init (InitEvent x).
 Proof using.
-  done.
+  unfold is_init; auto.
 Qed.
 
 (******************************************************************************)
-(** ** Same tid restriction *)
+(* ** Same tid restriction *)
 (******************************************************************************)
 
 Definition is_tid i a : Prop := tid a = i.
 
-Definition same_tid := (fun x y => tid x = tid y).
+Definition same_tid := (fun a b => tid a = tid b).
+
+Definition ext_sb a b := 
+  match a, b with
+  | (ThreadEvent t i _), (ThreadEvent t' j _) => t = t' /\ i < j
+  | (FpgaEvent _ i _), (FpgaEvent _ j _) => i < j
+  | (InitEvent _), (ThreadEvent _ _ _) => True
+  | (InitEvent _), (FpgaEvent _ _ _) => True
+  | _, _ => False
+end.
+
 
 Lemma restr_eq_rel_same_tid r :  restr_eq_rel tid r  ≡ r ∩ same_tid.
-Proof using. unfold same_tid; basic_solver. Qed.
+Proof using. unfold same_tid.  basic_solver. Qed.
 
 Lemma funeq_same_tid (r: relation Event) (H: funeq tid r):
  r ⊆ r ∩ same_tid.
@@ -117,20 +338,21 @@ Lemma same_loc_trans : transitive same_loc.
 Proof using. unfold same_loc; red; ins. by rewrite H. Qed.
 
 Lemma same_loc_sym : symmetric same_loc.
-Proof using. unfold same_loc; red; ins. Qed.
+Proof using. unfold same_loc; red; ins.
+Qed.
 
 (******************************************************************************)
 (** ** Values and locations getters  *)
 (******************************************************************************)
 
-Lemma exists_valw a : exists vw, valw a = vw.
+(* Lemma exists_valw a : exists vw, valw a = vw.
 Proof using. unfold valw; desc; eexists; eauto. Qed.
 
 Lemma exists_valr a : exists vw, valr a = vw.
 Proof using. unfold valr; desc; eexists; eauto. Qed.
 
 Lemma exists_loc a : exists x, loc a = x.
-Proof using. unfold loc; desc; eexists; eauto. Qed.
+Proof using. unfold loc; desc; eexists; eauto. Qed. *)
 
 
 (******************************************************************************)
@@ -139,18 +361,22 @@ Proof using. unfold loc; desc; eexists; eauto. Qed.
 
 Definition same_index := (fun x y => index x = index y).
 
-Definition ext_sb a b := 
-  match a, b with 
-    | _, InitEvent _ => False
-    | InitEvent _, ThreadEvent _ _ _ => True
-    | ThreadEvent t i _, ThreadEvent t' i' _ => t = t' /\ i < i' 
-   end.
+(* Definition ext_sb a b := 
+  match a, b with
+  | (ThreadEvent t i _), (ThreadEvent t' j _) => t = t' /\ i < j
+  | (FpgaEvent _ i _), (FpgaEvent _ j _) => i < j
+  | (InitEvent _), (ThreadEvent _ _ _) => True
+  | (InitEvent _), (FpgaEvent _ _ _) => True
+  | _, _ => False
+end. *)
+
+(* Definition same_index := (fun x y => index x = index y). *)
+
 
 Lemma ext_sb_trans : transitive ext_sb.
 Proof using.
 unfold ext_sb; red; ins.
-destruct x,y,z; ins; desf; splits; eauto.
-by rewrite H2.
+destruct x,y,z; ins; desf; splits; eauto; lia.
 Qed.
 
 Lemma ext_sb_irr : irreflexive ext_sb.
@@ -173,6 +399,7 @@ destruct x,y,z; ins; desf.
 cut(index1 < index2 \/ index2 < index1).
 tauto.
 lia.
+lia.
 Qed.
 
 Lemma ext_sb_semi_total_r x y z 
@@ -183,7 +410,7 @@ unfold ext_sb in *.
 destruct x,y,z; ins; desf; eauto.
 cut(index1 < index2 \/ index2 < index1).
 tauto.
-lia.
+lia. lia.
 Qed.
 
 Lemma ext_sb_tid_init x y (SB : ext_sb x y): tid x = tid y \/ is_init x.
@@ -203,6 +430,8 @@ Proof using.
   cut (index0 < index1 \/ index1 < index0 \/ index0 = index1).
   ins; desf; eauto 10.
   lia.
+  cut (index0 < index1 \/ index1 < index0 \/ index0 = index1).
+  ins; desf; eauto 10. lia.
 Qed.
 
 Lemma tid_n_init_ext_sb: same_tid ⨾ ⦗set_compl is_init⦘ ⊆ same_index ∪ ext_sb ∪ ext_sb⁻¹.
@@ -212,19 +441,27 @@ Proof using.
   basic_solver 12.
 Qed.
 
-End Events.
+Lemma ext_sb_index x y (SB: ext_sb x y) (N: ~ is_init x): index x < index y.
+Proof.
+  unfold ext_sb in *; desf; ins; desf; eauto.
+Qed.
 
 (******************************************************************************)
 (** ** Tactics *)
 (******************************************************************************)
 
+
+
+End Events. 
+
+
 #[global]
-Hint Unfold set_union set_inter is_r is_w is_rmw : type_unfolderDb.
-#[global]
+Hint Unfold set_union set_inter is_cpu_rd is_cpu_wr is_cpu_fence is_wr_req is_wr_resp is_fence_req_one is_fence_resp_one is_fence_req_all is_fence_resp_all is_rd_req is_rd_resp : type_unfolderDb.
+(* #[global]
 Hint Unfold is_r_l is_w_l is_rmw_l : type_unfolderDb.
 Tactic Notation "type_unfolder" :=  repeat autounfold with type_unfolderDb in *.
 
 Tactic Notation "type_solver" int_or_var(index) := 
   type_unfolder; basic_solver index.
 
-Tactic Notation "type_solver" :=  type_solver 4.
+Tactic Notation "type_solver" :=  type_solver 4. *)
